src/concurrency/DNS.Worker.Minimal.fst
@@ -6,12 +6,134 @@ open LowStar.Modifies
 open Steel.Memory
 open Steel.ST.Util
 open DNS.QUIC.StreamMapping
+module EPR = DNS.Protocol.Parser.EverParseRuntime
+module CAST = FStar.Int.Cast
 
 let noerror_response_flags_hi (request_flags_hi:FStar.UInt8.t) : FStar.UInt8.t =
   FStar.UInt8.logor 0x80uy (FStar.UInt8.logand request_flags_hi 0x79uy)
 
 let noerror_response_flags_lo (request_flags_lo:FStar.UInt8.t) : FStar.UInt8.t =
   FStar.UInt8.logand request_flags_lo 0x10uy
+
+val scan_uncompressed_qname_length :
+  request_buffer:buffer FStar.UInt8.t ->
+  request_len:FStar.UInt32.t ->
+  pos:FStar.UInt32.t ->
+  consumed:FStar.UInt32.t ->
+  Stack (n:FStar.UInt32.t{FStar.UInt32.v n <= 255})
+    (requires (fun h0 ->
+      live h0 request_buffer /\
+      FStar.UInt32.v request_len <= LowStar.Buffer.length request_buffer /\
+      FStar.UInt32.v request_len <= 271 /\
+      FStar.UInt32.v pos <= FStar.UInt32.v request_len /\
+      FStar.UInt32.v consumed <= 255))
+    (ensures (fun h0 _ h1 -> modifies_none h0 h1))
+    (decreases (FStar.UInt32.v request_len - FStar.UInt32.v pos))
+
+let rec scan_uncompressed_qname_length request_buffer request_len pos consumed =
+  if FStar.UInt32.gte pos request_len then
+    0ul
+  else
+    begin
+      assert (FStar.UInt32.v pos < LowStar.Buffer.length request_buffer);
+      let label_len_byte = LowStar.Buffer.index request_buffer pos in
+      let label_len = CAST.uint8_to_uint32 label_len_byte in
+      if FStar.UInt32.eq label_len 0ul then
+        if FStar.UInt32.lt consumed 255ul then
+          begin
+            assert (FStar.UInt32.v consumed + 1 < 4294967296);
+            FStar.UInt32.add consumed 1ul
+          end
+        else
+          0ul
+      else if FStar.UInt32.gt label_len 63ul then
+        0ul
+      else
+        begin
+          assert (FStar.UInt32.v label_len <= 63);
+          assert (FStar.UInt32.v pos <= FStar.UInt32.v request_len);
+          assert (FStar.UInt32.v request_len <= 271);
+          assert (FStar.UInt32.v pos + 1 + FStar.UInt32.v label_len < 4294967296);
+          assert (FStar.UInt32.v consumed + 1 + FStar.UInt32.v label_len < 4294967296);
+          let step = FStar.UInt32.add 1ul label_len in
+          let next_pos = FStar.UInt32.add pos step in
+          let next_consumed = FStar.UInt32.add consumed step in
+          if FStar.UInt32.gt next_pos request_len ||
+             FStar.UInt32.gt next_consumed 255ul then
+            0ul
+          else
+            begin
+              assert (FStar.UInt32.v next_pos <= FStar.UInt32.v request_len);
+              assert (FStar.UInt32.v next_pos > FStar.UInt32.v pos);
+              assert (FStar.UInt32.v next_consumed <= 255);
+              scan_uncompressed_qname_length
+                request_buffer
+                request_len
+                next_pos
+                next_consumed
+            end
+        end
+    end
+
+val validate_minimal_uncompressed_question_request :
+  request_buffer:buffer FStar.UInt8.t ->
+  request_len:FStar.UInt32.t ->
+  Stack bool
+    (requires (fun h0 ->
+      live h0 request_buffer /\
+      FStar.UInt32.v request_len <= LowStar.Buffer.length request_buffer))
+    (ensures (fun h0 _ h1 -> modifies_none h0 h1))
+
+let validate_minimal_uncompressed_question_request request_buffer request_len =
+  if FStar.UInt32.lt request_len 17ul ||
+     FStar.UInt32.lt 271ul request_len then
+    false
+  else
+    begin
+      assert (FStar.UInt32.v request_len >= 17);
+      assert (11 < LowStar.Buffer.length request_buffer);
+      let qd_hi = LowStar.Buffer.index request_buffer 4ul in
+      let qd_lo = LowStar.Buffer.index request_buffer 5ul in
+      let an_hi = LowStar.Buffer.index request_buffer 6ul in
+      let an_lo = LowStar.Buffer.index request_buffer 7ul in
+      let ns_hi = LowStar.Buffer.index request_buffer 8ul in
+      let ns_lo = LowStar.Buffer.index request_buffer 9ul in
+      let ar_hi = LowStar.Buffer.index request_buffer 10ul in
+      let ar_lo = LowStar.Buffer.index request_buffer 11ul in
+      if FStar.UInt8.eq qd_hi 0x00uy &&
+         FStar.UInt8.eq qd_lo 0x01uy &&
+         FStar.UInt8.eq an_hi 0x00uy &&
+         FStar.UInt8.eq an_lo 0x00uy &&
+         FStar.UInt8.eq ns_hi 0x00uy &&
+         FStar.UInt8.eq ns_lo 0x00uy &&
+         FStar.UInt8.eq ar_hi 0x00uy &&
+         FStar.UInt8.eq ar_lo 0x00uy then
+        let qname_length =
+          scan_uncompressed_qname_length request_buffer request_len 12ul 0ul in
+        assert (FStar.UInt32.v qname_length <= 255);
+        assert (FStar.UInt32.v qname_length + 16 < 4294967296);
+        let expected_request_len = FStar.UInt32.add qname_length 16ul in
+        if FStar.UInt32.eq qname_length 0ul ||
+           not (FStar.UInt32.eq expected_request_len request_len) then
+          false
+        else
+          begin
+            assert (FStar.UInt32.v qname_length > 0);
+            assert (FStar.UInt32.v qname_length <= 255);
+            assert (12 <= LowStar.Buffer.length request_buffer);
+            assert (12 <= FStar.UInt32.v request_len);
+            let question_len = FStar.UInt32.sub request_len 12ul in
+            let question = LowStar.Buffer.offset request_buffer 12ul in
+            let validation_code =
+              EPR.check_dns_uncompressed_question_code
+                qname_length
+                question
+                question_len in
+            not (FStar.UInt8.eq validation_code 0uy)
+          end
+      else
+        false
+    end
 
 val prepare_worker_minimal_error_response_send :
   ctx_ptr:buffer stream_context ->
@@ -136,3 +258,42 @@ let prepare_worker_empty_noerror_response_send
       LowStar.Buffer.upd response_buffer 11ul 0x00uy;
       12ul
     end
+
+val prepare_worker_validated_minimal_response_send :
+  ctx_ptr:buffer stream_context ->
+  response_buffer:buffer FStar.UInt8.t ->
+  response_capacity:FStar.UInt32.t ->
+  request_len:FStar.UInt32.t ->
+  ST FStar.UInt32.t
+    (requires (fun h0 ->
+      live h0 ctx_ptr /\
+      LowStar.Buffer.length ctx_ptr >= 1 /\
+      live h0 response_buffer /\
+      FStar.UInt32.v response_capacity <= LowStar.Buffer.length response_buffer /\
+      (let ctx = FStar.Seq.index (LowStar.Buffer.as_seq h0 ctx_ptr) 0 in
+       live h0 ctx.sc_buf /\
+       FStar.UInt32.v request_len <= LowStar.Buffer.length ctx.sc_buf)))
+    (ensures (fun h0 _ h1 ->
+      modifies (loc_buffer response_buffer) h0 h1 /\
+      live h1 response_buffer))
+
+let prepare_worker_validated_minimal_response_send
+  ctx_ptr
+  response_buffer
+  response_capacity
+  request_len =
+  let s = LowStar.Buffer.index ctx_ptr 0ul in
+  let valid =
+    validate_minimal_uncompressed_question_request s.sc_buf request_len in
+  if valid then
+    prepare_worker_empty_noerror_response_send
+      ctx_ptr
+      response_buffer
+      response_capacity
+      request_len
+  else
+    prepare_worker_minimal_error_response_send
+      ctx_ptr
+      response_buffer
+      response_capacity
+      request_len
